\documentclass[12pt]{article}
\usepackage{amsmath, amssymb, setspace}
\usepackage{newtxtext,newtxmath}
\usepackage{titlesec}
\usepackage{fancyhdr}
\usepackage{times} 
\usepackage{graphicx}
\usepackage{xcolor}
\usepackage[dvipsnames]{xcolor}
\setstretch{1.12}
\usepackage[top=1cm, left=1.2in, right=1.4in]{geometry}
\pagestyle{fancy}
\fancyhf{}
\cfoot{2019-20}
\renewcommand{\headrulewidth}{2pt} 
\renewcommand{\headrule}{{\color{cyan}\hrule width\headwidth height\headrulewidth}} 

\fancyhead[L]{\includegraphics[width=5cm,height=2cm]{COMET.jpeg}} 
\fancyhead[C]{\textcolor{MidnightBlue}{\Large\textbf{NCERT \vspace{0.3em} \\ \large Task-3}}}
\fancyhead[R]{\textcolor{MidnightBlue}{K SATHVIKA \\ COMET.FWC20}}
\setlength{\headheight}{4.5cm}
\setlength{\headsep}{10pt}

\titleformat{\section}
  {\normalfont\Large\bfseries}{\thesection}{1em}{}

\begin{document}
 \textbf{Note that we have found the roots of $2x^2 - 5x + 3 = 0$ by factorising $2x^2 - 5x + 3$ into two linear factors and equating each factor to zero.}

\vspace{1em}

\noindent \textcolor{cyan}{\textbf{Example 4 :}} Find the roots of the quadratic equation $6x^2 - x - 2 = 0$.\\
\textcolor{cyan}{\textbf{Solution :}} We have
\[
6x^2 - x - 2 = 6x^2 + 3x - 4x - 2
\]
\[
\quad\quad\quad\quad\quad = 3x(2x + 1) - 2(2x + 1)
\]
\[
\quad\quad\quad\quad\quad = (3x - 2)(2x + 1)
\]

The roots of $6x^2 - x - 2 = 0$ are the values of $x$ for which $(3x - 2)(2x + 1) = 0$ \\
Therefore, $3x - 2 = 0$ or $2x + 1 = 0$,

\[
\text{i.e.,} \quad x = \frac{2}{3} \quad \text{or} \quad x = -\frac{1}{2}
\]

Therefore, the roots of $6x^2 - x - 2 = 0$ are $\frac{2}{3}$ and $-\frac{1}{2}$.

\vspace{1em}

We verify the roots, by checking that $\frac{2}{3}$ and $-\frac{1}{2}$ satisfy $6x^2 - x - 2 = 0$.

\vspace{1em}

\noindent \textcolor{cyan}{\textbf{Example 5 :}} Find the roots of the quadratic equation $3x^2 - 2\sqrt{6}x + 2 = 0$.\\
\textcolor{cyan}{\textbf{Solution :}} 
\[
3x^2 - 2\sqrt{6}x + 2 = 3x^2 - \sqrt{6}x - \sqrt{6}x + 2
\]
\[
\quad = \sqrt{3}x(\sqrt{3}x - \sqrt{2}) - \sqrt{2}(\sqrt{3}x - \sqrt{2})
\]
\[
\quad = (\sqrt{3}x - \sqrt{2})(\sqrt{3}x - \sqrt{2})
\]

So, the roots of the equation are the values of $x$ for which
\[
(\sqrt{3}x - \sqrt{2})(\sqrt{3}x - \sqrt{2}) = 0
\]

Now, $\sqrt{3}x - \sqrt{2} = 0$ for $x = \frac{\sqrt{2}}{\sqrt{3}}$

So, this root is repeated twice, one for each repeated factor $\sqrt{3}x - \sqrt{2}$.

\vspace{1em}

Therefore, the roots of $3x^2 - 2\sqrt{6}x + 2 = 0$ are $\dfrac{\sqrt{2}}{\sqrt{3}}, \dfrac{\sqrt{2}}{\sqrt{3}}$.
\vspace{2cm}
\begin{center}
2019-20
\end{center}

\end{document}
